Foundation/Modal/ModalCompanion/Standard/Int.lean
@@ -3,12 +3,11 @@ module
 public import Foundation.Logic.Embedding
 public import Foundation.Modal.Boxdot.GL_Grz
 public import Foundation.Modal.ModalCompanion.Standard.Basic
-public import Foundation.Propositional.Hilbert.Standard
-public import Foundation.Propositional.Kripke.Logic.Int
+public import Foundation.Propositional.Kripke.Hilbert.Int.Basic
 
 @[expose] public section
 
-namespace LO.Modal
+namespace LO
 
 open LO.Entailment LO.Entailment.FiniteContext LO.Modal.Entailment
 open Propositional
@@ -17,102 +16,48 @@ open Propositional.Logic (smallestMC largestMC)
 open Modal
 open Modal.Kripke
 
-lemma Kripke.sound_frameClass_of_equiv (L₁ L₂ : Logic ℕ) [L₁ ≊ L₂] {C : Kripke.FrameClass} [Sound L₁ C] : Sound L₂ C := by grind;
-lemma Kripke.complete_frameClass_of_equiv (L₁ L₂ : Logic ℕ) [L₁ ≊ L₂] {C : Kripke.FrameClass} [Complete L₁ C] : Complete L₂ C := by grind;
+namespace Propositional.Int
+
+lemma provable_S4_of_mem : φ ∈ Propositional.Int → Modal.S4 ⊢ φᵍ := by
+  apply Propositional.Hilbert.provable_gödelTranslated_of_mem_logic;
+  rintro _ ⟨φ, ⟨_, rfl⟩, rfl⟩;
+  simp;
+
+theorem modalCompanion_S4 : ModalCompanion Propositional.Int Modal.S4 := by
+  apply modalCompanion_via_kripkeSemantics (P := λ _ => True);
+  . apply provable_S4_of_mem;
+  . intro φ;
+    apply Hilbert.Int.instKripkeComplete.complete;
+  . rintro φ hφ F _ _;
+    apply Modal.S4.instSoundLogicNatFormulaFrameClassS4.sound;
+    . grind;
+    . apply Set.mem_setOf_eq.mpr;
+      exact {};
+
+lemma provable_Grz_of_mem : φ ∈ Propositional.Int → Modal.Grz ⊢ φᵍ := fun h ↦ WeakerThan.pbl $ provable_S4_of_mem h
+
+theorem modalCompanion_Grz : ModalCompanion Propositional.Int Modal.Grz := by
+  apply modalCompanion_via_kripkeSemantics (P := λ {κ} _ => Finite κ);
+  . apply provable_Grz_of_mem;
+  . intro φ;
+    apply Hilbert.Int.instKripkeCompleteFinite.complete;
+  . rintro φ hφ F _ _;
+    apply Modal.instSoundLogicNatFormulaFrameClassGrzFinite_Grz.sound;
+    . grind;
+    . apply Set.mem_setOf_eq.mpr;
+      exact {};
+
+end Propositional.Int
 
 
-lemma gS4_of_Int : Propositional.Int ⊢ φ → Modal.S4 ⊢ φᵍ := by
-  apply provable_gödelTranslated_of_provable;
-  rintro _ ⟨φ, ⟨_⟩, ⟨s, rfl⟩⟩;
-  apply nec! $ efq!;
+/-
+namespace Propositional.Cl
 
-namespace S4
-
-instance : Modal.S4 ≊ Propositional.Int.smallestMC := by
-  apply Logic.equiv_of_provable;
-  intro φ;
-  constructor;
-  . intro hφ;
-    induction hφ using Modal.Hilbert.Normal.rec! with
-    | axm _ h => rcases h with (rfl | rfl | rfl) <;> simp;
-    | mdp ihφψ ihψ => exact ihφψ ⨀ ihψ;
-    | nec ihφ => exact nec! ihφ;
-    | _ => apply Logic.sumNormal.mem₁!; simp;
-  . intro hφ;
-    induction hφ using Logic.sumNormal.rec! with
-    | subst ih => apply Logic.subst _ ih;
-    | mdp ihφψ ihψ => exact ihφψ ⨀ ihψ;
-    | nec ih => apply nec! ih;
-    | mem₁ h => tauto;
-    | mem₂ h =>
-      rcases h with ⟨φ, hφ, rfl⟩;
-      apply gS4_of_Int;
-      simpa [theory, Propositional.Logic.iff_provable, Set.mem_setOf_eq] using hφ;
-
-lemma eq_smallestMC_of_Int : Modal.S4 = Propositional.Int.smallestMC := Logic.eq_of_equiv
-
-instance : Sound Propositional.Int.smallestMC FrameClass.S4 := Kripke.sound_frameClass_of_equiv Modal.S4 Propositional.Int.smallestMC
-
-instance : ModalCompanion Propositional.Int Modal.S4 := by
-  apply eq_smallestMC_of_Int ▸
-    Modal.instModalCompanion_of_smallestMC_via_KripkeSemantics
-    Propositional.Kripke.FrameClass.all
-    FrameClass.S4;
-  intro F _;
-  constructor;
-
-instance : Entailment.FaithfullyEmbeddable Propositional.Int Modal.S4 :=
-  ModalCompanion.tofaithfullyEmbeddable _ _
-
-end S4
-
-
-
-
-instance : Propositional.Int.smallestMC ⪯ Modal.Grz := calc
-  _ ≊ Modal.S4  := by symm; infer_instance;
-  _ ⪯ Modal.Grz := inferInstance
-
-
-namespace Grz
-
-instance : Modal.Grz ≊ Propositional.Int.largestMC := by
-  apply Logic.equiv_of_provable;
-  intro φ;
-  constructor;
-  . intro hφ;
-    induction hφ using Modal.Hilbert.Normal.rec! with
-    | axm _ h => rcases h with (rfl | rfl) <;> simp;
-    | mdp ihφψ ihψ => exact ihφψ ⨀ ihψ;
-    | nec ihφ => exact nec! ihφ;
-    | _ => apply Logic.sumNormal.mem₁!; simp;
-  . intro hφ;
-    induction hφ using Logic.sumNormal.rec! with
-    | mdp ihφψ ihψ => exact ihφψ ⨀ ihψ;
-    | subst ih => apply Logic.subst _ ih;
-    | nec ih => apply nec! ih;
-    | mem₁ h => apply WeakerThan.pbl h;
-    | mem₂ h => rcases h with ⟨φ, hφ, rfl⟩; simp;
-
-lemma is_largestMC_of_Int : Modal.Grz = Propositional.Int.largestMC := Logic.eq_of_equiv
-
-instance : Sound Propositional.Int.largestMC FrameClass.finite_Grz := Kripke.sound_frameClass_of_equiv Modal.Grz Propositional.Int.largestMC
-
-instance : ModalCompanion Propositional.Int Modal.Grz := by
-  apply is_largestMC_of_Int ▸ Modal.instModalCompanion_of_largestMC_via_KripkeSemantics
-    Propositional.Kripke.FrameClass.finite_all
-    FrameClass.finite_Grz
-  rintro F hF;
-  simp_all only [Set.mem_setOf_eq];
-  exact {}
-
-end Grz
-
-
-lemma iff_provable_Cl_provable_dia_gS4 : Propositional.Cl ⊢ φ ↔ Modal.S4 ⊢ ◇φᵍ := by
+lemma iff_mem_S4_dia : φ ∈ Propositional.Cl ↔ Modal.S4 ⊢ ◇φᵍ := by
   constructor;
   . intro h;
     suffices Modal.S4 ⊢ □◇φᵍ by exact axiomT'! this;
+    have := glivenko.mpr h;
     have : Modal.S4 ⊢ (∼∼φ)ᵍ := ModalCompanion.companion.mp $ glivenko.mpr h;
     cl_prover [this];
   . intro h;
@@ -121,6 +66,12 @@ lemma iff_provable_Cl_provable_dia_gS4 : Propositional.Cl ⊢ φ ↔ Modal.S4 �
     replace h : Modal.S4 ⊢ □◇φᵍ := nec! h;
     cl_prover [h];
 
+end Propositional.Cl
+-/
+
+end LO
+
+/-
 /--
   Chagrov & Zakharyaschev 1997, Theorem 3.89
 -/
@@ -129,6 +80,6 @@ theorem embedding_Int_GL : Propositional.Int ⊢ φ ↔ Modal.GL ⊢ φᵍᵇ:=
 
 instance : Entailment.FaithfullyEmbeddable Propositional.Int Modal.GL where
   prop := ⟨(·ᵍᵇ), fun _ ↦ embedding_Int_GL.symm⟩
+-/
 
-end LO.Modal
 end
